LeanYjs/Network/CausalOrder.lean
@@ -36,6 +36,13 @@ inductive hb_consistent : List A → Prop where
       (∀ b, b ∈ ops → ¬ b ≤ a) →
       hb_consistent (a :: ops)
 
+inductive hb_strong_consistent : List A → List A → Prop where
+  | nil : hb_strong_consistent ops []
+  | cons : ∀ (a : A) (ops₀ ops₁ : List A),
+      hb_strong_consistent (a :: ops₀) ops₁ →
+      (∀b, b < a → b ∈ ops₀) →
+      hb_strong_consistent ops₀ (a :: ops₁)
+
 theorem List.sublist_mem {A : Type} {l₁ l₂ : List A} (h_sublist : l₁ <+ l₂) {a : A} :
   a ∈ l₁ → a ∈ l₂ := by
   intros h_mem
@@ -139,20 +146,42 @@ omit [DecidableEq A] [Operation A] in theorem hb_consistent_concurrent (a : A) (
       | inr h_mem_tail =>
         apply ih h_consistent_tail h_mem_tail
 
-theorem hb_concurrent_foldr {ops₀ ops₁ : List A} :
+inductive compatibleOps [DecidableEq A] (hb : CausalOrder A) : Operation.State A → List A → Prop where
+  | nil : compatibleOps hb s []
+  | cons :
+      compatibleOp hb s a →
+      effect a s = Except.ok s' →
+      compatibleOps hb s' ops' →
+      compatibleOps hb s (a :: ops')
+
+theorem hb_concurrent_foldr {ops₀ ops₁ : List A} {s : Operation.State A} :
   concurrent_commutative hb (ops₀ ++ a :: ops₁) →
   (∀ x ∈ ops₀, hb_concurrent hb x a) →
-  List.foldr (effect_comp (A := A)) (effect a ▷ init) (List.map (fun a => effect a) ops₀) =
-  effect a ▷ List.foldr (effect_comp (A := A)) init (List.map (fun a => effect a) ops₀) := by
+  compatibleOps hb s (ops₀ ++ a :: ops₁) →
+  List.foldr (effect_comp (A := A)) (effect a ▷ init) (List.map (fun a => effect a) ops₀) s =
+  (effect a ▷ List.foldr (effect_comp (A := A)) init (List.map (fun a => effect a) ops₀)) s := by
   induction ops₀ with
   | nil =>
     simp
   | cons b bs ih =>
-    intro h_comm h_concurrent
+    intro h_comm h_concurrent hcompatible
     simp
+    symm
+    calc
+      _ = ((effect a ▷ effect b) ▷ (foldr effect_comp init (map (fun a => effect a) bs))) s := by rw [effect_comp_assoc]
+      _ = ((effect a ▷ effect b) s >>= (foldr effect_comp init (map (fun a => effect a) bs))) := by rfl
+      _ = ((effect b ▷ effect a) s >>= (foldr effect_comp init (map (fun a => effect a) bs))) := by
+        rw [h_comm a b] <;> try grind [hb_concurrent]
+        simp [hb_concurrent] at *
+        grind
+        
+
+
+
     rw [ih]
     . rw [←effect_comp_assoc]
       have h_effect_b_effect_a_comm : effect b ▷ effect a = effect a ▷ effect b := by
+        ext s
         apply h_comm
         . simp
         . simp
@@ -167,24 +196,17 @@ theorem hb_concurrent_foldr {ops₀ ops₁ : List A} :
         right; assumption
     . intros; apply h_concurrent; simp; right; assumption
 
-def compatibleOps [DecidableEq A] (s : Operation.State A) (ops : List A) : Prop :=
-  ∀ op ∈ ops, ∃ops',
-    hb_consistent hb ops' ∧
-    (∀ a, a < op → a ∈ ops') ∧
-    (∀ a ∈ ops', ¬op ≤ a) ∧
-    (ops'.map (fun a => effect a) |> List.foldr effect_comp Except.pure) Operation.init = Except.ok s
-
 theorem effect_comp_apply {op1 op2 : Effect (A := A)} {s : Operation.State A} :
   effect_comp op1 op2 s = op1 s >>= op2 := by
   rfl
 
-theorem hb_consistent_effect_convergent (ops₀ ops₁ : List A) (init : Effect)
+theorem hb_consistent_effect_convergent (ops₀ ops₁ : List A) (init : Effect) s
   (h_consistent₀ : hb_consistent hb ops₀)
   (h_consistent₁ : hb_consistent hb ops₁)
+  (hcompatible₀ : compatibleOps hb s ops₀)
+  (hcompatible₁ : compatibleOps hb s ops₁)
   (h_commutative : concurrent_commutative hb ops₀)
-  (no_dup₀ : ops₀.Nodup) (no_dup₁ : ops₁.Nodup)
-  (s : Operation.State A)
-  (h_compatible : compatibleOps hb s ops₀) :
+  (no_dup₀ : ops₀.Nodup) (no_dup₁ : ops₁.Nodup) :
   (∀ a, a ∈ ops₀ ↔ a ∈ ops₁) →
   (ops₀.map (fun a => effect a) |> List.foldr effect_comp init) s =
   (ops₁.map (fun a => effect a) |> List.foldr effect_comp init) s :=
@@ -210,25 +232,29 @@ by
       . -- Case a = b
         simp [effect_comp]
         rw [h_eq]
-        apply bind_congr
-        intros x
-        apply ih
-        . apply hb_consistent_tail hb a ops₀ h_consistent₀
-        . apply hb_consistent_tail hb b ops₁ h_consistent₁
-        . intros a b h_a_mem h_b_mem h_concurrent
-          apply h_commutative
-          . simp; right; assumption
-          . simp; right; assumption
-          . assumption
-        . simp at no_dup₀
-          obtain ⟨ h_no_dup₀ ⟩ := no_dup₀
-          assumption
-        . simp at no_dup₁
-          obtain ⟨ h_no_dup₁ ⟩ := no_dup₁
-          assumption
-        . sorry
-        . subst h_eq
-          apply List.no_dup_cons_eq _ h_mem no_dup₀ no_dup₁
+        have (eq := hx) x := effect b s; rw [<-hx]
+        cases x with
+        | error e => rfl
+        | ok x =>
+          simp [bind, Except.bind.eq_2]
+          apply ih
+          . apply hb_consistent_tail hb a ops₀ h_consistent₀
+          . apply hb_consistent_tail hb b ops₁ h_consistent₁
+          . cases hcompatible₀; grind
+          . cases hcompatible₁; grind
+          . intros a b h_a_mem h_b_mem h_concurrent
+            apply h_commutative
+            . simp; right; assumption
+            . simp; right; assumption
+            . assumption
+          . simp at no_dup₀
+            obtain ⟨ h_no_dup₀ ⟩ := no_dup₀
+            assumption
+          . simp at no_dup₁
+            obtain ⟨ h_no_dup₁ ⟩ := no_dup₁
+            assumption
+          . subst h_eq
+            apply List.no_dup_cons_eq _ h_mem no_dup₀ no_dup₁
       . -- Case a ≠ b
         have ⟨ ops₁_first, ops₁_last, h_ops₁_eq ⟩ : ∃ ops₁_first ops₁_last, ops₁ = ops₁_first ++ a :: ops₁_last := by
           have h_a_mem_ops₁ : a ∈ ops₁ := by
@@ -316,11 +342,14 @@ by
           | ok s' =>
             simp [bind, Except.bind.eq_2]
             rw [ih (b :: ops₁_first ++ ops₁_last)]
-            simp
+            . simp
             . cases h_consistent₀
               assumption
             . apply hb_consistent_sublist _ h_consistent₁
               simp
+            . cases hcompatible₀; grind
+            . cases hcompatible₁
+
             . intros x y h_x_mem h_ey_mem h_concurrent
               apply h_commutative
               simp; right; assumption
@@ -331,10 +360,10 @@ by
               assumption
             . apply Nodup.sublist _ no_dup₁
               simp
-            . intros op h_op_mem
-              obtain ⟨ ops', hops' ⟩ := h_compatible op (by simp [h_op_mem])
-              use ops' ++ [a]
-              sorry
+            -- . intros op h_op_mem
+            --   obtain ⟨ ops', hops' ⟩ := h_compatible op (by simp [h_op_mem])
+            --   use ops' ++ [a]
+            --   sorry
             . intros x
               constructor
               . intro h_mem₀
@@ -355,7 +384,7 @@ by
         . simp [hb_concurrent] at *
           obtain ⟨ h_not_le_ab, h_not_le_ba ⟩ := h_a_b_concurrent
           constructor <;> assumption
-        . apply h_compatible _ (by grind)
-        . apply h_compatible _ (by grind)
+        . cases hcompatible₁; grind
+        . cases hcompatible₀; grind
 
 end CausalOrder
